theories/lang/notation.v
@@ -46,6 +46,8 @@ Notation "e1 |{ ot1 , ot2 } e2" := (BinOp OrOp ot1 ot2 e1%E e2%E)
   (at level 70, format "e1  |{ ot1 ,  ot2 }  e2") : expr_scope.
 Notation "e1 ^{ ot1 , ot2 } e2" := (BinOp XorOp ot1 ot2 e1%E e2%E)
   (at level 70, format "e1  ^{ ot1 ,  ot2 }  e2") : expr_scope.
+Notation "e1 ,{ ot1 , ot2 } e2" := (BinOp Comma ot1 ot2 e1%E e2%E)
+  (at level 30, format "e1  ,{ ot1 ,  ot2 }  e2") : expr_scope.
 (* The offset must be evaluated first for the type system to work, thus the order is switched here. *)
 Notation "e1 'at_offset{' ly , ot1 , ot2 } e2" := (BinOp (PtrOffsetOp ly) ot2 ot1 e2%E e1%E)
   (at level 70, format "e1  at_offset{ ly ,  ot1 ,  ot2 }  e2") : expr_scope.
